src/model/Reserves.v
@@ -1,0 +1,232 @@
+Require Import RelationClasses.
+
+From sflib Require Import sflib.
+
+From PromisingLib Require Import Axioms.
+From PromisingLib Require Import Basic.
+From PromisingLib Require Import DataStructure.
+From PromisingLib Require Import Loc.
+From PromisingLib Require Import Language.
+From PromisingLib Require Import Event.
+
+Require Import Time.
+
+Set Implicit Arguments.
+
+
+Module Reserves.
+  Definition t := Loc.t -> option Time.t.
+
+  Definition eq := @eq t.
+
+  Definition le (lhs rhs: t): Prop :=
+    forall loc ts (LHS: lhs loc = Some ts),
+      rhs loc = Some ts.
+
+  Global Program Instance le_PreOrder: PreOrder le.
+  Next Obligation. ii. ss. Qed.
+  Next Obligation. ii. eauto. Qed.
+  #[global] Hint Resolve le_PreOrder_obligation_2: core.
+
+  Lemma antisym l r
+        (LR: le l r)
+        (RL: le r l):
+    l = r.
+  Proof.
+    extensionality loc.
+    specialize (LR loc). specialize (RL loc).
+    destruct (l loc) eqn:L, (r loc) eqn:R; eauto.
+    exploit LR; eauto.
+  Qed.
+
+  Definition bot: t := fun _ => None.
+
+  Lemma bot_spec (tm:t): le bot tm.
+  Proof.
+    ii. ss.
+  Qed.
+
+  Definition disjoint (x y: t): Prop :=
+    forall loc ts1 ts2
+      (GET1: x loc = Some ts1)
+      (GET2: y loc = Some ts2),
+      False.
+
+  Global Program Instance disjoint_Symmetric: Symmetric disjoint.
+  Next Obligation.
+    ii. eauto.
+  Qed.
+
+  Lemma bot_disjoint prom: disjoint bot prom.
+  Proof.
+    ii. ss.
+  Qed.
+
+  Definition finite (rsv: t): Prop :=
+    exists dom,
+    forall loc ts (GET: rsv loc = Some ts),
+      List.In loc dom.
+
+  Lemma bot_finite: finite bot.
+  Proof.
+    exists []. ss.
+  Qed.
+
+  
+  Variant add (rsv1: t) (loc: Loc.t) (ts: Time.t) (rsv2: t): Prop :=
+  | add_intro
+      (GET: rsv1 loc = None)
+      (RSV2: rsv2 = LocFun.add loc (Some ts) rsv1)
+  .
+
+  Variant remove (rsv1: t) (loc: Loc.t) (ts: Time.t) (rsv2: t): Prop :=
+  | remove_intro
+      (GET: rsv1 loc = Some ts)
+      (RSV2: rsv2 = LocFun.add loc None rsv1)
+  .
+
+  Variant reserve (rsv1 grsv1: t) (loc: Loc.t) (ts: Time.t) (rsv2 grsv2: t): Prop :=
+  | reserve_intro
+      (RSV: add rsv1 loc ts rsv2)
+      (GRSV: add grsv1 loc ts grsv2)
+  .
+
+  Variant cancel (rsv1 grsv1: t) (loc: Loc.t) (ts: Time.t) (rsv2 grsv2: t): Prop :=
+  | cancel_intro
+      (RSV: remove rsv1 loc ts rsv2)
+      (GRSV: remove grsv1 loc ts grsv2)
+  .
+
+
+  Lemma add_o
+        rsv2 rsv1 loc ts l
+        (ADD: add rsv1 loc ts rsv2):
+    rsv2 l = if Loc.eq_dec l loc then Some ts else rsv1 l.
+  Proof.
+    inv ADD. unfold LocFun.add. ss.
+  Qed.
+
+  Lemma add_get0
+        rsv1 loc ts rsv2
+        (ADD: add rsv1 loc ts rsv2):
+    (<<GET1: rsv1 loc = None>>) /\
+    (<<GET2: rsv2 loc = Some ts>>).
+  Proof.
+    inv ADD. split; ss.
+    unfold LocFun.add. condtac; ss.
+  Qed.
+
+  Lemma add_get1
+        rsv1 loc ts rsv2 l ts'
+        (ADD: add rsv1 loc ts rsv2)
+        (GET: rsv1 l = Some ts'):
+    rsv2 l = Some ts'.
+  Proof.
+    inv ADD. unfold LocFun.add. condtac; ss. subst. congr.
+  Qed.
+
+  Lemma add_finite
+        rsv1 loc ts rsv2
+        (ADD: add rsv1 loc ts rsv2)
+        (FINITE: finite rsv1):
+    finite rsv2.
+  Proof.
+    inv ADD. inv FINITE.
+    exists (loc :: x). unfold LocFun.add. intro.
+    condtac; ss; eauto.
+  Qed.
+
+  Lemma remove_o
+        rsv2 rsv1 loc ts l
+        (REMOVE: remove rsv1 loc ts rsv2):
+    rsv2 l = if Loc.eq_dec l loc then None else rsv1 l.
+  Proof.
+    inv REMOVE. unfold LocFun.add. ss.
+  Qed.
+
+  Lemma remove_get0
+        rsv1 loc ts rsv2
+        (REMOVE: remove rsv1 loc ts rsv2):
+    (<<GET1: rsv1 loc = Some ts>>) /\
+    (<<GET2: rsv2 loc = None>>).
+  Proof.
+    inv REMOVE. split; ss.
+    unfold LocFun.add. condtac; ss.
+  Qed.
+
+  Lemma remove_get1
+        rsv1 loc ts rsv2 l ts'
+        (REMOVE: remove rsv1 loc ts rsv2)
+        (GET: rsv1 l = Some ts'):
+    (<<LOC: l = loc>>) \/
+    (<<GET2: rsv2 l = Some ts'>>).
+  Proof.
+    inv REMOVE. unfold LocFun.add. condtac; auto.
+  Qed.
+
+  Lemma remove_finite
+        rsv1 loc ts rsv2
+        (REMOVE: remove rsv1 loc ts rsv2)
+        (FINITE: finite rsv1):
+    finite rsv2.
+  Proof.
+    inv REMOVE. inv FINITE.
+    exists x. unfold LocFun.add. intro.
+    condtac; ss; eauto.
+  Qed.
+
+  Lemma reserve_le
+        rsv1 grsv1 loc ts rsv2 grsv2
+        (RESERVE: reserve rsv1 grsv1 loc ts rsv2 grsv2)
+        (LE1: le rsv1 grsv1):
+    le rsv2 grsv2.
+  Proof.
+    ii. revert LHS.
+    inv RESERVE. inv RSV. inv GRSV.
+    unfold LocFun.add. condtac; ss. eauto.
+  Qed.
+
+  Lemma cancel_le
+        rsv1 grsv1 loc ts rsv2 grsv2
+        (CANCEL: cancel rsv1 grsv1 loc ts rsv2 grsv2)
+        (LE1: le rsv1 grsv1):
+    le rsv2 grsv2.
+  Proof.
+    ii. revert LHS.
+    inv CANCEL. inv RSV. inv GRSV.
+    unfold LocFun.add. condtac; ss. eauto.
+  Qed.
+
+  Lemma reserve_disjoint
+        rsv1 grsv1 loc ts rsv2 grsv2
+        ctx
+        (RESERVE: reserve rsv1 grsv1 loc ts rsv2 grsv2)
+        (LE_CTX: le ctx grsv1)
+        (DISJOINT: disjoint rsv1 ctx):
+    (<<DISJOINT: disjoint rsv2 ctx>>) /\
+    (<<LE_CTX: le ctx grsv2>>).
+  Proof.
+    inv RESERVE. inv RSV. inv GRSV. splits; ii.
+    - revert GET1. unfold LocFun.add.
+      condtac; ss; subst; eauto. i. clarify.
+      exploit LE_CTX; eauto. i. congr.
+    - unfold LocFun.add. condtac; ss; eauto. clarify.
+      exploit LE_CTX; eauto. i. congr.
+  Qed.
+
+  Lemma cancel_disjoint
+        rsv1 grsv1 loc ts rsv2 grsv2
+        ctx
+        (CANCEL: cancel rsv1 grsv1 loc ts rsv2 grsv2)
+        (LE_CTX: le ctx grsv1)
+        (DISJOINT: disjoint rsv1 ctx):
+    (<<DISJOINT: disjoint rsv2 ctx>>) /\
+    (<<LE_CTX: le ctx grsv2>>).
+  Proof.
+    inv CANCEL. inv RSV. inv GRSV. splits; ii.
+    - revert GET1. unfold LocFun.add.
+      condtac; ss; subst; eauto.
+    - unfold LocFun.add. condtac; ss; subst; eauto.
+      exploit DISJOINT; eauto. ss.
+  Qed.
+End Reserves.
